IO.Effect.fst
@@ -6,16 +6,16 @@ open ExtraTactics
 open Common
 open IO.Free
 
-(** The postcondition for an io computation is defined over the 
+(** The postcondition for an io computation is defined over the
 result (type: a + exn) and local trace (type: trace).
-The local trace represents the events that happend during the 
+The local trace represents the events that happend during the
 computation. Local trace is in chronological order.
 
 We also have the history (type: trace) which represents the
 events that happend until the beggining of the io computation.
-The history is reverse chronology order. 
+The history is reverse chronology order.
 
-At the end of an io computation, the trace will be 
+At the end of an io computation, the trace will be
 (reverse of local trace) appended to the history. **)
 
 let io_post a = maybe a -> lt:trace -> Type0  // local_trace (from old to new)
@@ -28,26 +28,26 @@ let io_return_wp (a:Type) (x:a) : io_wpty a =
 unfold
 let compute_post (a b:Type) (h:trace) (kw : a -> io_wpty b) (p:io_post b)
   : io_post a =
-      (fun result local_trace -> 
+      (fun result local_trace ->
         match result with
         | Inl result -> (
             kw result
-            ((List.rev local_trace) @ h) 
-            (fun result' local_trace' -> 
+            ((List.rev local_trace) @ h)
+            (fun result' local_trace' ->
                 p result' (local_trace @ local_trace')))
         | Inr err -> p (Inr err) local_trace)
 
 unfold
 let io_bind_wp (a:Type) (b:Type) (w : io_wpty a) (kw : a -> io_wpty b) : io_wpty b =
-  fun h p -> 
+  fun h p ->
     w h (compute_post a b h kw p)
 
-let gen_post #a (post:io_post a) (e:event) = 
+let gen_post #a (post:io_post a) (e:event) =
   fun x local_trace -> post x (e :: local_trace)
 
 let rec io_interpretation #a
-  (m : io a) 
-  (p : io_post a) : Type0 = 
+  (m : io a)
+  (p : io_post a) : Type0 =
   match m with
   | Return x -> p (Inl x) []
   | Throw err -> p (Inr err) []
@@ -60,7 +60,7 @@ let rec io_interpretation #a
 // REFINED COMPUTATION MONAD (repr)
 let io_irepr (a:Type) (wp:io_wpty a) =
   // TODO: more intuition about this? why does this look like a
-  // reader monad? 
+  // reader monad?
   h:trace -> post:io_post a ->
     Pure (io a)
       (requires (wp h post))
@@ -75,8 +75,8 @@ let io_wpty_ord wp1 wp2 = forall h p. wp1 h p ==> wp2 h p
 
 let io_ibind (a b : Type) (wp_v : io_wpty a) (wp_f: a -> io_wpty b) (v : io_irepr a wp_v)
   (f : (x:a -> io_irepr b (wp_f x))) : io_irepr b (io_bind_wp _ _ wp_v wp_f) =
-  fun h p -> 
-    let t = (io_bind a b 
+  fun h p ->
+    let t = (io_bind a b
         (v h (compute_post a b h wp_f p))
         (fun x ->
           assume (wp_f x h p);
@@ -116,25 +116,25 @@ let lift_pure_iowp (a:Type) (wp:pure_wp a) (f:(eqtype_as_type unit -> PURE a wp)
 
 sub_effect PURE ~> IOwp = lift_pure_iowp
 
-let throw (err:exn) : IOwp trace (fun _ p -> p (Inr err) []) =
-  IOwp?.reflect(fun _ _ -> io_throw _ err)
+let throw (#a:Type) (err:exn) : IOwp a (fun _ p -> p (Inr err) []) =
+  IOwp?.reflect(fun _ _ -> io_throw a err)
 
 let static_cmd
   (pi : monitorable_prop)
   (cmd : io_cmds)
   (argz : io_args cmd) :
-  IOwp 
-    (res cmd) 
-    (fun h p -> 
+  IOwp
+    (res cmd)
+    (fun h p ->
       (** precondition **)
       pi h (| cmd, argz |) /\
       (forall (r:io_resm cmd) lt. (
       (** postcondition **)
-        ~(Inr? r /\ Inr?.v r == Contract_failure) /\ 
+        ~(Inr? r /\ Inr?.v r == Contract_failure) /\
         lt == [convert_call_to_event cmd argz r] /\
         enforced_locally pi h lt) ==>  p r lt)) =
   IOwp?.reflect(fun _ _ -> io_call cmd argz)
-  
+ 
 effect IO
   (a:Type)
   (pi : monitorable_prop)
@@ -142,9 +142,9 @@ effect IO
   (post : trace -> maybe a -> trace -> Type0) =
   IOwp a (fun (h:trace) (p:io_post a) ->
     enforced_globally pi h /\
-    pre h /\ 
+    pre h /\
     (forall res lt. (
       enforced_globally pi (apply_changes h lt) /\
       post h res lt ==>  p res lt)))
 
-// let fd = static_cmd pi Openfile "../Makefile" 
+// let fd = static_cmd pi Openfile "../Makefile"
